

Name - Sajal Nandor

Section - C

Roll No. - 2022 UG 3022

Maths Assignment V

1. Form the P.D.E for the given solutions.

(i) $z = f(x^2 + y^2)$

Sol. $z_x = f'(x^2 + y^2) \cdot 2x$ - (i)

$z_y = f'(x^2 + y^2) \cdot 2y$ - (ii)

Eq (i) $\times y$ - Eq (ii) $\times x \Rightarrow \boxed{yz_x - xz_y = 0}$

(ii) $f(xyz, x^2 + y^2 + z^2) = 0$

Sol. $U = xyz$ $V = x^2 + y^2 + z^2$

$P = J\left(\frac{U, V}{x, y, z}\right) = \begin{vmatrix} \frac{\partial U}{\partial x} & \frac{\partial V}{\partial x} \\ \frac{\partial U}{\partial y} & \frac{\partial V}{\partial y} \end{vmatrix} = \begin{vmatrix} yz & 2x \\ xz & 2y \end{vmatrix} \Rightarrow 2xz^2 - 2xy^2$

$Q = J\left(\frac{U, V}{z, x}\right) = \begin{vmatrix} \frac{\partial U}{\partial z} & \frac{\partial V}{\partial z} \\ \frac{\partial U}{\partial x} & \frac{\partial V}{\partial x} \end{vmatrix} = \begin{vmatrix} xy & 2z \\ yz & 2x \end{vmatrix} = 2y(x^2 - z^2)$

$R = J\left(\frac{U, V}{x, y}\right) = \begin{vmatrix} \frac{\partial U}{\partial x} & \frac{\partial V}{\partial x} \\ \frac{\partial U}{\partial y} & \frac{\partial V}{\partial y} \end{vmatrix} = \begin{vmatrix} yz & 2x \\ xz & 2y \end{vmatrix} \Rightarrow 2z(y^2 - x^2)$

The P.D.E is given by

$Pp + Qq = R$

$\boxed{2x(z^2 - y^2)p + 2y(x^2 - z^2)q = 2z(y^2 - x^2)}$

(iii) $ax^2 + by^2 + z^2 = 1$

$2ax + 2z z_x = 0$ - (i) $\Rightarrow z_x = -\frac{ax}{z}$

$2by + 2z z_y = 0$ - (ii) $\Rightarrow z_y = -\frac{by}{z}$

Eq (i) $\times by$ - Eq (ii) $\times ax \Rightarrow byz_x - axz_y = -\frac{aby}{z} + \frac{aby}{z}$

$\Rightarrow \boxed{byz_x - axz_y = 0}$

$$(iv) (x-h)^2 + (y-k)^2 + z^2 = a^2$$

$$\text{Sol. } 2(x-h) + 2z z_x = 0 \quad \text{--- (i)}$$

$$z_x = \frac{x-h}{z}$$

$$2(y-k) + 2z z_y = 0 \quad \text{--- (ii)}$$

$$z_y = \frac{y-k}{z}$$

$$\text{eqn (i)} \times (y-k) - \text{eqn (ii)} \times (x-h) = \boxed{(y-k)z_x - (x-h)z_y = 0}$$

$$(v) xyz = g(x+y+z)$$

$$\text{Sol. } yz x_x = g'(x+y+z)$$

$$x z_x z = \frac{g(x+y+z)}{xy}$$

$$z_x = \frac{g'(x+y+z)}{yz} = \frac{g(x+y+z)}{xyz} \Rightarrow z_x(1 - xyz g'(x+y+z)) = \frac{g(x+y+z)}{x}$$

$$z_y = \frac{g'(x+y+z)}{xz} = \frac{g(x+y+z)}{xyz} \Rightarrow z_y(1 - xyz g'(x+y+z)) = \frac{g(x+y+z)}{y}$$

$$\text{eqn (i)} \times x - \text{eqn (ii)} \times y =$$

$$\Rightarrow \boxed{x z_x - y z_y = 0}$$

$$i) g\left(\frac{1}{x} - \frac{1}{y}, \frac{xy}{z}\right) = 0$$

$$u = \frac{1}{x} - \frac{1}{y} \quad v = \frac{xy}{z}$$

$$p = \frac{J(u,v)}{(y,z)} = \begin{vmatrix} \frac{\partial u}{\partial y} & \frac{\partial u}{\partial z} \\ \frac{\partial v}{\partial y} & \frac{\partial v}{\partial z} \end{vmatrix} = \begin{vmatrix} -\frac{1}{y^2} & \frac{x}{z} \\ 0 & -\frac{xy}{z^2} \end{vmatrix} \Rightarrow \boxed{-\frac{x}{yz^2}}$$

$$q = \frac{J(u,v)}{(z,x)} = \begin{vmatrix} \frac{\partial u}{\partial z} & \frac{\partial u}{\partial x} \\ \frac{\partial v}{\partial z} & \frac{\partial v}{\partial x} \end{vmatrix} = \begin{vmatrix} 0 & -\frac{xy}{z^2} \\ -\frac{1}{xz} & \frac{y}{x} \end{vmatrix} \Rightarrow \boxed{-\frac{y}{xz^2}}$$

$$R = \frac{J(u,v)}{(x,y)} = \begin{vmatrix} \frac{\partial u}{\partial x} & \frac{\partial u}{\partial y} \\ \frac{\partial v}{\partial x} & \frac{\partial v}{\partial y} \end{vmatrix} = \begin{vmatrix} -\frac{1}{x^2} & \frac{y}{z} \\ \frac{1}{xy^2} & \frac{x}{z} \end{vmatrix} \Rightarrow -\frac{1}{x^2} - \frac{1}{zy} \Rightarrow -\frac{1}{z} \left(\frac{1}{x} + \frac{1}{y} \right) = \frac{-(x+y)}{xyz}$$

$$p p + q q = R$$

$$\frac{-x}{yz^2} p + \frac{-y}{xz^2} q = \frac{-(x+y)}{xyz} \Rightarrow \frac{x}{y} p + \frac{y}{x} q = \frac{x+y}{x}$$

$$\Rightarrow \boxed{x^2 p + y^2 q = y(x+y)}$$

Classify the following PDE's as Linear, Semilinear and Quasilinear.

(i) $p + q = xyz + x$

Ans. Linear, Semilinear, Quasilinear

(ii) $xp + yq = z^2 + yx$

Ans. Linear, Semilinear, Quasilinear

(iii) $xp + y^2q = xz^2 + xy$

Ans. Semilinear, Quasilinear

(iv) $xzp + yq = xyz + y^2$

2) Q. 2) Ans. Quasilinear.

Classify the following PDE's as Hyperbolic, Parabolic and Elliptic.

i) $x^2 \frac{\partial^2 u}{\partial t^2} - \frac{\partial^2 u}{\partial x^2} = u$

Ans. $B = 0$, $A = x^2$, $C = -1$

$$B^2 - 4AC = 0 - 4(x^2)(-1) = 4x^2 > 0$$

Hyperbolic

ii) $tU_{tt} + 2U_{xt} + xU_{xx} + U_t = 0$

Ans. $B = 2$, $A = t$, $C = x$

$$B^2 - 4AC = 4 - 4xt = 4(1 - xt)$$

Ans. Hyperbolic if $xt < 1$

Parabolic if $xt = 1$

Elliptic if $xt > 1$

iii) $xU_{tt} + tU_{xt} + U_{tt} = 0$

Ans. $A = x$, $B = t$, $C = 1$

$$B^2 - 4AC = t^2 - 4x$$

Hyperbolic if $t^2 - 4x > 0$

Parabolic if $t^2 = 4x$

Elliptic if $t^2 - 4x < 0$

$$(iv) x^2 u_{tt} + 30xt + 20x_{xx} + 170t = 100x$$

$$\text{Sol. } A = x^2, \quad B = 3, \quad C = x$$

$$B^2 - 4ac = 9 - 4x^3$$

$$\text{Hyperbolic if } 9 - 4x^3 > 0$$

$$\text{Parabolic if } 9 - 4x^3 = 0$$

$$\text{Elliptic if } 9 - 4x^3 < 0$$

$$(v) u_{tt} + t u_{xt} + x u_{xx} + 20t + u_x + 6u = 0$$

$$\text{Sol. } A = 1, \quad B = t, \quad C = x$$

$$B^2 - 4ac = t^2 - 4x$$

$$\text{Hyperbolic if } t^2 - 4x > 0$$

$$\text{Parabolic if } t^2 - 4x = 0$$

$$\text{Elliptic if } t^2 - 4x < 0$$

4. Solve the first order Quasilinear PDE's :

$$(i) p \tan x + q \tan y = \tan z$$

$$\text{Sol. } \frac{dx}{\tan x} = \frac{dy}{\tan y} = \frac{dz}{\tan z}$$

$$\int \frac{dx}{\tan x} = \int \frac{dy}{\tan y}$$

$$\int \frac{dy}{\tan y} = \int \frac{dz}{\tan z} + C_2$$

$$C_2 = \ln |\sin y| - \ln |\sin z|$$

$$C_2 = \frac{\sin y}{\sin z}$$

$$3) \int \frac{\cos x}{\sin x} dx = \int \frac{\cos y}{\sin y} dy + C_1$$

$$u = \sin x$$

$$du = \cos x dx$$

$$v = \sin y$$

$$dv = \cos y dy$$

$$\int \frac{du}{u} = \int \frac{dv}{v} + C_1$$

$$\ln |\sin x| = \ln |\sin y| + C_1$$

$$C_1 = \ln \left| \frac{\sin x}{\sin y} \right|$$

$$C_1 = \ln \left| \frac{\sin x}{\sin y} \right|$$

$$u = C_1 = \frac{\sin x}{\sin y}$$

$$v = C_2 = \frac{\sin y}{\sin z}$$

$$\phi \left(\frac{\sin x}{\sin y}, \frac{\sin y}{\sin z} \right) = 0$$

$$(y-z)p + (x-y)q = z-x$$

$$\frac{dx}{y-z} = \frac{dy}{x-y} = \frac{dz}{z-x}$$

$$\frac{dx+dy+dz}{y-z+x-y+z-x} = 0$$

$$dx+dy+dz = 0$$

$$\boxed{x+y+z = C_1}$$

$$\frac{xdy + ydz + zdz}{xy-zx+xz-yz+zy-xy} = 1$$

$$xdy + ydz + zdz = 0$$

$$\frac{x^2}{2} + yz + zy = C_2$$

$$\boxed{x^2 + 4yz = C_2}$$

$$\phi(x+y+z, x^2+4yz) = 0$$

$$ii) p + 3q = 5z + \tan(y-3x)$$

$$\frac{dx}{1} = \frac{dy}{3} = \frac{dz}{5 + \tan(y-3x)}$$

$$dx = \frac{dy}{3}$$

$$3x = y + C_1$$

$$\boxed{C_1 = y - 3x}$$

$$\frac{dx}{1} = \frac{dz}{5 + \tan(C_1)}$$

$$5 + \tan(C_1) dx = dz$$

$$5x + \tan(y-3x)x = z + C_2$$

$$C_2 = x(5 + \tan(y-3x)) - z$$

$$\phi(y-3x, x(5 + \tan(y-3x)) - z) = 0$$

$$i) xp - yq + x^2 - y^2 = 0$$

$$x^2 + px = y^2 + qy = 0$$

$$p = \frac{a-x^2}{x} \quad q = \frac{a-y^2}{y}$$

$$dz = p dx + q dy$$

$$z = \int \frac{a-x^2}{x} dx + \int \frac{a-y^2}{y} dy$$

$$z = \int \frac{a}{x} dx + \int x dx + \int \frac{a}{y} dy - \int y dy$$

$$z = a \ln x - \frac{x^2}{2} + a \ln y - \frac{y^2}{2}$$

$$z = a \ln\left(\frac{x}{y}\right) - \frac{1}{2}(x^2 + y^2)$$

$$(V) (z^2 - 2yz - y^2)p + (xy + zx)q = xy - zx$$

$$\text{Sol. } \frac{dz}{z^2 - 2yz - y^2} = \frac{dy}{xy + zx} = \frac{dz}{xy - zx}$$

$$\frac{xdy + ydy + zdy}{x^2z - 2xyz - y^2z + xy^2 + xyz + xy^2} = 1$$

$$\frac{x^2z - 2xyz - y^2z + xy^2 + xyz + xy^2}{x^2z - 2xyz - y^2z + xy^2 + xyz + xy^2} = 1$$

$$\frac{x^2}{2} + \frac{y^2}{2} + \frac{z^2}{2} = C_1$$

$$C_1 = x^2 + y^2 + z^2$$

$$\frac{dy - dz}{2zx} = \frac{dy + dz}{2xy}$$

$$\frac{dy - dz}{2} = \frac{dy + dz}{\frac{dy}{dz}}$$

$$\int ydy - \int ydz = \int zdy + \int zdz$$

$$\frac{y^2}{2} - \int ydz = \int zdy + \frac{z^2}{2}$$

$$\frac{y^2}{2} - \frac{z^2}{2} = \int d(yz)$$

$$y^2 - z^2 = 2yz + C_1$$

$$y^2 - z^2 - 2yz = C_2$$

$$\phi(x^2 + y^2 + z^2, y^2 - z^2 - 2yz) = 0$$

Solve the first order non-linear PDEs:

1) $q - p + x - y = 0$

2) $p - x = q - y = a$

$p = a + x, \quad q = a + y$

$dz = p dx + q dy$

$dz = (a+x)dx + (a+y)dy$

$z = ax + \frac{x^2}{2} + ay + \frac{y^2}{2} + C$

3) $\sqrt{p} + \sqrt{q} = 2x$

$\sqrt{p} - 2x + -\sqrt{q} + 0 = a$

$\sqrt{p} = a + 2x, \quad \sqrt{q} = -a$

$p = (a+2x)^2, \quad q = a^2$

$dz = p dx + q dy$

$dz = (a^2 + 4ax + 4x^2)dx + a^2 dy$

$z = a^2 x + \frac{4x^3}{3} + 2ax^2 + a^2 y + C$

4) $p^2 + q^2 = z(x+y)$

5) $zx + zy = p^2 + q^2$

$z = \frac{p^2}{x+y} + \frac{q^2}{x+y}$

$p = a, \quad q = b$

$z = \frac{a^2 + b^2}{x+y}$

6) $z = px + qy + p^2 + q^2$

This is Clairaut's form.

$p = a, \quad q = b$

$z = ax + by + a^2 + b^2$

$$(V) x^2 p^2 + y^2 q^2 = z^2$$

$$\text{Sol. } z^2 - x^2 p^2 + y^2 q^2 = 0$$

$$q = ap$$

$$\Rightarrow x^2 p^2 + a^2 y^2 p^2 = z^2$$

$$\frac{dz}{z} = \frac{z}{\sqrt{x^2 + a^2 y^2}}$$

$$dz = p(dx + a dy)$$

$$\frac{dz}{z} = \frac{1}{\sqrt{x^2 + a^2 y^2}} (x + ay)$$

$$\Rightarrow \log z = (x + ay) \int \frac{1}{\sqrt{x^2 + a^2 y^2}}$$

$$\Rightarrow z = e^{x+ay} \cdot e^{\sqrt{x^2 + a^2 y^2}}$$

$$(vi) pq = 1$$

$$p = a, \quad q = g(p)$$

$$\Rightarrow q = \frac{1}{p} = g(p)$$

$$dz = p dx + q dy$$

$$z = \int a dx + \int \frac{1}{a} dy + c$$

$$z = ax + \frac{y}{a} + c$$

$$(vii) p^2 + q^2 = 1$$

$$\text{Sol. let } p = a, \quad q = \pm \sqrt{1 - a^2}$$

$$dz = p dx + q dy$$

$$z = \int a dx \pm \int \sqrt{1 - a^2} dy$$

$$z = ax \pm \sqrt{1 - a^2} y + c$$

Solve the higher order PDEs:

$$(D^3 - 4D^2D' + 3DD'^3)z = 0$$

It is non homogeneous -

$F(D, D')$ is not reducible to linear factors

$$C.F. = \sum A e^{hxy}$$

$$\text{where } h^3 - 4h^2k + 3hk^3 = 0$$

$$(D^4 - 2D^3D' + 2DD'^3 - D'^4)z = 0$$

Putting $D \rightarrow m$, $D' \rightarrow 1$

$$A.E. \quad m^4 - 2m^3 + 2m - 1$$

$m=1$ is one solution

$$\Rightarrow (m-1)(m^3 - m^2 - m + 1)$$

$$\Rightarrow (m-1)(m+1)(m^2 - 2m + 1)$$

$$\Rightarrow (m-1)(m+1)(m-1)^2, \Rightarrow m=1, 1, 1, m=-1$$

$$C.F. = \phi_1(y-x) + \phi_2(y+x) + x\phi_3(y+x) + x^2\phi_4(y+x)$$

$$(D^4 + D'^4)z = 0$$

Putting $D \rightarrow m$, $D' \rightarrow 1$

$$A.E. \quad m^4 + 1 = 0 \Rightarrow (m^2+1)^2 - 2m^2$$

$$m^4 = -1 \Rightarrow (m^2+1-\sqrt{2}m)(m^2+1+\sqrt{2}m) = 0$$

$$m^2 = \pm i \Rightarrow m^2+1-\sqrt{2}m = 0, \quad m^2+\sqrt{2}m+1 = 0$$

$$m = \frac{\sqrt{2} \pm \sqrt{2-4}}{2}, \quad m = \frac{-\sqrt{2} \pm \sqrt{2-4}}{2}$$

$$m = \frac{\sqrt{2} \pm \sqrt{2-4}}{2}$$

$$m = \sqrt{2} \pm \sqrt{2}i$$

$$m = -\sqrt{2} \pm \sqrt{2}i$$

$$m = \sqrt{2}(1+i), \sqrt{2}(1-i), \sqrt{2}(-1+i), \sqrt{2}(-1-i)$$

$$C.F. = \phi_1(y + \sqrt{2}(1+i)x) + \phi_2(y + \sqrt{2}(1-i)x) + \phi_3(y + \sqrt{2}(-1+i)x) + \phi_4(y + \sqrt{2}(-1-i)x)$$

$$(iv) (D^4 + D^4 - 2D^2 D'^2)z = 0$$

$$\text{Sol. } D \rightarrow m, D' \rightarrow 1$$

$$\text{A.E. } m^4 + 1 - 2m^2 = 0$$

$$m^4 - 2m^2 + 1 = 0$$

$$(m^2 - 1)^2 = 0$$

$$m = \pm 1, m = \pm 1$$

$$\text{C.F.} = \phi_1(y+x) + x\phi_2(y+x) + \phi_3(y-x) + x\phi_4(y-x)$$

$$(v) (D + D' - 2)(D + 4D' - 3)z = 0$$

$$\text{Sol. } D \rightarrow m, D' \rightarrow 1$$

$$(m+1-2)(m+4-3) = 0$$

$$(m-1)(m+1) = 0$$

$$m = 1, m = -1$$

$$\text{C.F.} = \phi_1(y+x) + \phi_2(y-x)$$

$$(vi) (D + 3D' + 4)^2 z = 0$$

$$\text{Sol. } D \rightarrow m, D' \rightarrow 1$$

$$(m+3+4)^2 = 0$$

$$(m+7)^2 = 0$$

$$m = -7, -7$$

$$\text{C.F.} = \phi_1(y-7x) + x\phi_2(y-7x)$$

$$(vii) x - D + p - q = 0$$

$$\text{Sol. } D^2 - D'^2 + D - D' = 0$$

$$D \rightarrow m, D' \rightarrow 1$$

$$m^2 - 1 + m - 1 = 0$$

$$m^2 + m - 2 = 0$$

$$(m+2)(m-1) = 0$$

$$m = 1, m = -2$$

$$\text{C.F.} = \phi_1(y+x) + \phi_2(y-2x)$$

$$(D^2 - 4DD' + 4D'^2)z = e^{2x+y}$$

A.E. $D \rightarrow m, D' \rightarrow 1$

$$m^2 - 4m + 4 = 0$$

$$\therefore (m-2)^2 = 0$$

$$\boxed{m = 2, 2}$$

$$C.F. = \phi_1(y+2x) + x\phi_2(y+2x)$$

$$P.I. = \frac{1}{F(D, D')} \phi(ax+by)$$

$$= \frac{1}{F(2,1)} \int$$

$$F(2,1) = 4 - 8 + 4 = 0$$

$$F'(2,1) = 2D - 4D' \Big|_{2,1} = 4 - 4 = 0$$

$$F''(2,1) = \boxed{2}$$

$$P.I. = \frac{x^2}{2} e^{2x+y}$$

$$z = C.F. + P.I.$$

$$z = \phi_1(y+2x) + x\phi_2(y+2x) + \frac{x^2}{2} e^{2x+y}$$

$$(X) (D^2 - D'^2 - 2D + 2D')z = e^{2x+3y}$$

Sol. A.E. $D \rightarrow m, D' \rightarrow 1$

$$m^2 - 1 - 2m + 2 = 0$$

$$m^2 - 2m + 1 = 0$$

$$(m-1)^2 = 0$$

$$m = 1, 1$$

$$C.F. = \phi_1(y+x) + x\phi_2(y+x)$$

$$P.I. = \frac{1}{F(D, D')} e^{2x+3y}$$

$$F(2,3) = 4 - 9 - 4 + 6 = 10 - 13 = -3$$

$$P.I. = \frac{1}{F(2,3)} \int e^u du \Big|_{u=2x+3y}$$

$$P.I. = -\frac{1}{3} e^{2x+3y}$$

$$z = C.F. + P.I.$$

$$z = \phi_1(y+x) + x\phi_2(y+x) - \frac{e^{2x+3y}}{3}$$

$$(X) (D^2 + 2DD' + D'^2) z = \sin(2x + 3y)$$

$$\text{Sol. A.E. } D \rightarrow m, D' \rightarrow 1$$

$$m^2 + 2m + 1 = 0$$

$$(m+1)^2 = 0$$

$$m = -1, -1$$

$$\text{C.F.} = \phi_1(y-x) + x \phi_2(y-x)$$

$$\text{P.I.} = \frac{1}{F(D, D')} \iint \phi(u) du \Big|_{u=2x+3y}$$

$$F(2,3) = 4 + 2 \times 2 \times 3 + 3^2$$

$$= 4 + 12 + 9$$

$$= 25$$

$$\text{P.I.} = \frac{1}{25} \int \sin u du \Big|_{u=2x+3y}$$

$$\text{P.I.} = -\frac{1}{25} \cos(2x+3y)$$

$$z = \phi_1(y-x) + x \phi_2(y-x) - \frac{1}{25} \cos(2x+3y)$$

$$(Xi) (D+1)(D+D'-1)z = \sin(x+2y)$$

$$\text{Sol. A.E. } D \rightarrow m, D' \rightarrow 1$$

$$(m+1)(m+1-1) = 0$$

$$m = 0, m = -1$$

$$\text{C.F.} = \phi_1(y) + \phi_2(y-x)$$

$$\text{P.I.} = \frac{1}{F(D, D')} \int \phi(u) du \Big|_{u=x+2y}$$

$$F(1,2) = (1+1)(1+2-1) = 2(2) = 4$$

$$\text{P.I.} = \frac{1}{4} \int \sin u du \Big|_{u=x+2y}$$

$$\text{P.I.} = -\frac{\cos(x+2y)}{4}$$

$$z = \phi_1(y) + \phi_2(y-x) - \frac{\cos(x+2y)}{4}$$

$$x) (D^3 - 7DD' - 6D'^2)z = \sin(x+2y) + e^{3x+y}$$

$$\text{A.E. } D \rightarrow m, D' \rightarrow 1$$

$$m^3 - 7m - 6 = 0$$

$$(m+1)(m^2 - m - 6) = 0$$

$$(m+1)(m+2)(m-3) = 0$$

$$m = -1, -2, 3$$

$$\text{C.F.} = \phi_1(y-x) + \phi_2(y-2x) + \phi_3(y+3x)$$

$$\text{P.I.} = \frac{1}{F(0,0)} \sin(x+2y) + \frac{1}{F(0,1)} \int e^{3x+y}$$

$$F(1,2) = 1 - 28 - 48$$

$$= -75$$

$$= \frac{1}{-75} \int \sin u \, du \Big|_{u=x+2y} + \frac{1}{11} \int e^u \, du \Big|_{u=3x+y}$$

$$F(3,1) = 27 - 21 - 6$$

$$= 0$$

$$F'(3,1) = 27^2 - 7D' \Big|_{3,1}$$

$$= 18 - 7 = 11$$

$$= \frac{\cos(x+2y)}{-75} + \frac{x e^{3x+y}}{11}$$

$$z = \text{C.F.} + \text{P.I.}$$

$$z = \phi_1(y-x) + \phi_2(y-2x) + \phi_3(y+3x) + \frac{\cos(x+2y)}{-75} + \frac{x e^{3x+y}}{11}$$

$$\text{Xiii) } (4D^2 - 4DD' + D'^2)z = 16 \log(x+2y)$$

$$\text{A.E. } D \rightarrow m, D' \rightarrow 1$$

$$4m^2 - 4m + 1 = 0$$

$$(2m-1)^2 = 0$$

$$m = \frac{1}{2}, \frac{1}{2}$$

$$\text{C.F.} = \phi_1\left(y + \frac{x}{2}\right) + x \phi_2\left(y + \frac{x}{2}\right)$$

$$F(1,2) = 4 \times 1 - 4 \times 1 \times 2 + 2^2$$

$$= 4 - 8 + 4 = 0$$

$$\text{P.I.} = \frac{1}{F(0,0)} \int \phi(u) \, du \Big|_{\phi=x+2y}$$

$$F'(1,2) = 8D - 4D'$$

$$= 8 - 4 = 4$$

$$F''(1,2) = 8$$

$$\text{P.I.} = \frac{16}{8} \int \log(u) \, du \Big|_{u=x+2y}$$

$$\text{P.I.} = 2x^2 [\log u - 1]$$

$$\text{P.I.} = 2x^2 [(x+2y)(\log(x+2y) - 1)]$$

$$z = \phi_1\left(y + \frac{x}{2}\right) + x \phi_2\left(y + \frac{x}{2}\right) + 2x^2 [(x+2y)(\log(x+2y) - 1)]$$

$$(X \text{ (Xiv)}) (D^3 D' - 2DD'^2 + D'^3)z = x^{-2}$$

$$\text{A.E. } D' \rightarrow m, D \rightarrow 1$$

$$m^2 - 2m + 1 = 0$$

$$(m-1)^2 = 0$$

$$m = 1, 1$$

$$\text{C.F.} = \phi_1(y+x) + x\phi_2(y+x)$$

$$\text{P.I.} = \frac{1}{D^3 D'} x^{-2} y^0$$

$$\text{P.I.} = \frac{1}{(D^3 D' - 2DD'^2 + D'^3)} x^{-2} y^0$$

$$\text{P.I.} = \frac{1}{D^3} \left[1 - \frac{2D}{D'} + \frac{D^2}{D'^2} \right] x^{-2}$$

$$\text{P.I.} = \frac{1}{D^3} \left[\left(1 - \frac{2D}{D'} + \frac{D^2}{D'^2} \right) x^{-2} \right]$$

$$\text{P.I.} = \frac{1}{D^3} \left[\left(1 + \left(\frac{2D}{D'} - \frac{D^2}{D'^2} \right) - \left(\frac{2D}{D'} - \frac{D^2}{D'^2} \right)^2 + \left(\frac{2D}{D'} - \frac{D^2}{D'^2} \right)^3 \right) x^{-2} \right]$$

$$\text{P.I.} = \frac{1}{D^3} \left[\right]$$

$$\text{P.I.} = \frac{1}{D^3} \left[1 - \frac{(2DD' + D'^2)}{D'^2} \right] x^{-2}$$

$$\text{P.I.} = \frac{1}{D^3} \left[1 + \frac{2DD' + D'^2}{D'^2} - \frac{(2DD' + D'^2)^2}{D'^4} \right] x^{-2}$$

$$\text{P.I.} = \frac{1}{D^3} \left[x^{-2} + \frac{1}{D'^2} [2D'x - 2x^3 + 6x^{-4}] \right]$$

$$\text{P.I.} = \frac{1}{D^3} \left[x^{-2} + \frac{1}{D'^2} [-4x^{-3}y^0 + 6x^{-4}] \right]$$

$$\text{P.I.} = \frac{1}{D^3} [x^{-2} + 6x^{-4}y^2]$$

$$\text{P.I.} = x^{-2}y^3 + 6x^{-4}y^5$$

$$z = \phi_1(y+x) + x\phi_2(y+x) + x^{-2}y^3 + 6x^{-4}y^5$$

$$(D^3 - D^2)z = x^3 y^3$$

$$\text{A.E. } D \rightarrow m, \quad D^2 \rightarrow 1$$

$$m^3 - 1 = 0$$

$$m = 1, \omega, \omega^2$$

$$\text{C.F. } \phi_1(y+x) + \phi_2(y+\omega x) + \phi_3(y+\omega^2 x)$$

$$\text{P.I.} = \frac{1}{D^3 - D^2} x^3 y^3$$

$$= \frac{1}{D^2} \left[1 - \frac{D^2}{D^3} \right]^{-1} x^3 y^3$$

$$= \frac{1}{D^2} \left[1 + \frac{D^2}{D^3} + \frac{D^4}{D^6} + \dots \right] x^3 y^3$$

$$= \frac{1}{D^2} \left[x^3 y^3 + \frac{1}{D^3} x^3 y^3 \right]$$

$$= \frac{x^3 y^3}{4 \cdot 5 \cdot 6} + \frac{6 x^3}{4 \cdot 5 \cdot 6 \cdot 7 \cdot 8 \cdot 9} = \frac{x^3 y^3}{120} + \frac{x^3}{10080}$$

$$2. \text{ C.F. } + \text{ P.I.}$$

$$= \phi_1(y+x) + \phi_2(y+\omega x) + \phi_3(y+\omega^2 x) + \frac{x^3 y^3}{120} + \frac{x^3}{10080}$$

$$\text{Qvi) } (D^2 + 2DD' + D'^2)z = x^2 + xy + y^2$$

$$\text{A.E. } D \rightarrow m, \quad D' \rightarrow 1$$

$$m^2 + 2m + 1 = 0$$

$$(m+1)^2 = 0$$

$$m = -1, -1$$

$$\text{C.F.} = \phi_1(y-x) + x(y-x) + x^2 \phi_2(y-x)$$

$$\text{P.I.} = \frac{1}{D(D+1)^2} [x^2 + xy + y^2]$$

$$\text{P.I.} = \frac{1}{D^2 + 2DD' + D'^2} x^2 + \frac{1}{D^2 + 2DD' + D'^2} xy + \frac{1}{D^2 + 2DD' + D'^2} y^2$$

$$\text{P.I.} = \frac{1}{D^2} \left[1 + \frac{2D'}{D} + \frac{D'^2}{D^2} \right]^{-1} x^2 + \frac{1}{D^2} \left[1 + \frac{2D'}{D} + \frac{D'^2}{D^2} \right]^{-1} xy + \frac{1}{D^2} \left[1 + \frac{2D'}{D} + \frac{D'^2}{D^2} \right]^{-1} y^2$$

$$\text{P.I.} = \frac{1}{D^2} \left[1 - \frac{2DD' + D'^2}{D^2} + \frac{(2DD' + D'^2)^2}{D^4} \right] x^2 + \frac{1}{D^2} \left[1 + \frac{2DD' + D'^2}{D^2} \right] xy + \frac{1}{D^2} \left[1 + \frac{2DD' + D'^2}{D^2} \right] y^2$$

$$= \frac{1}{D^2} \left[x^2 - \frac{2}{D^2} \right] + \frac{1}{D^2} \left[xy + \frac{1}{D^2} [2] \right] + \frac{1}{D^2} \left[y^2 + \frac{1}{D^2} \right]$$

$$\Rightarrow \frac{1}{D^2}[x^2] + \frac{1}{D^2}[xy+x^2] + \frac{1}{D^2}[y^2]$$

$$\Rightarrow \frac{x^4}{12} + \frac{x^3y}{6} + \frac{y^4}{12}$$

$$Z = \phi_1(y-x) + x\phi_2(y-x) + \frac{x^4}{12} + \frac{x^3y}{6} + \frac{y^4}{12}$$

$$(XVII) \quad x - 4y = \frac{4x}{y^2} - \frac{y}{x^2}$$

$$\text{Sol. } D^2 - 4D' = \frac{4x}{y^2} - \frac{y}{x^2}$$

$$(D^2 - 4D')Z = 4xy^{-2} - yx^{-2}$$

$$\text{A.E. } \rightarrow D \rightarrow m, D' \rightarrow 1$$

$$m^2 - 4 = 0$$

$$m = \pm 2$$

$$\text{C.F.} = \phi_1(y+2x) + \phi_2(y-2x)$$

$$\text{P.I.} = \frac{1}{F(D, D')} \frac{4x}{y^2} 4xy^{-2} - \frac{1}{F(D, D')} \frac{y}{x^2}$$

$$\Rightarrow \frac{1}{D^2 - 4D^2} 4xy^{-2} - \frac{1}{D^2 - 4D} yx^{-2}$$

$$\Rightarrow \frac{1}{D^2} \left[1 - \frac{4D^2}{D^2} \right]^{-1} 4xy^{-2} - \frac{1}{(-4D^2)} \left[1 - \frac{D^2}{4D^2} \right]^{-1} yx^{-2}$$

$$\Rightarrow \frac{1}{D^2} \left[1 + \frac{4D^2}{D^2} - \frac{16D^4}{D^4} \right] 4xy^{-2} + \frac{1}{4D^2} \left[1 + \frac{D^2}{4D^2} - \frac{D^4}{16D^4} \right] yx^{-2}$$

$$\Rightarrow \frac{1}{D^2} \left[1 + \frac{4D^2}{D^2} - \frac{16D^4}{D^4} \right] yx^{-2} + \frac{1}{4D^2} \left[1 + \frac{D^2}{4D^2} - \frac{D^4}{16D^4} \right] 4xy^{-2}$$

$$\Rightarrow \frac{1}{D^2} [yx^{-2} + 0] + \frac{1}{4D^2} [4xy^{-2} + 0]$$

$$\Rightarrow -y \log x - x \log y$$

$$Z = \phi_1(y+2x) + \phi_2(y-2x) - (y \log x + x \log y)$$

$$(D^2 - D' + D + 3D' - 2)z = x^2y$$

$$\text{A.E. } D \rightarrow m, D' \rightarrow 1$$

$$m^2 - 1 + m + 3 - 2 = 0$$

$$m^2 + m = 0$$

$$m(m+1) = 0$$

$$m = 0, m = -1$$

$$\text{C.F.} = \phi_1(y) + \phi_2(y-x)$$

$$\text{P.I.} = \frac{1}{F(D, D')} x^2y$$

$$\text{P.I.} = \frac{1}{D^2 - D' + D + 3D' - 2} x^2y$$

$$\text{P.I.} = \frac{1}{D^2 \left[1 - \left(\frac{D^2}{D^2} - \frac{1}{D} - \frac{3D'}{D^2} + \frac{2}{D^2} \right) \right]} x^2y \quad \Rightarrow \quad \frac{1}{D^2 \left[1 - \left(\frac{D^2 - D - 3DD' + 2}{D^2} \right) \right]} x^2y$$

$$\text{P.I.} = \frac{1}{D^2} \left[1 - \left(\frac{D^2 - D - 3DD' + 2}{D^2} \right) \right]^{-1} x^2y \quad \Rightarrow$$

$$\Rightarrow \frac{1}{D^2} \left[1 + \frac{D^2 - D - 3DD' + 2}{D^2} + \frac{(D^2 - D - 3DD' + 2)^2}{D^4} \right] x^2y$$

$$\Rightarrow \frac{1}{D^2} \left[x^2y + \frac{1}{D^2} [0 + 2xy - 3x^2 + 2x^2y] \right] = \frac{1}{D^4} [0 + 2xy - 6x + 4xy + 6x + 6x^2 + 4xy - 6x^2 + 4x^2y]$$

$$\Rightarrow \frac{1}{D^2} \left[x^2y + \left[\frac{x^3y}{3} - \frac{x^4}{4} + \frac{x^4y}{6} \right] \right] =$$

$$\Rightarrow \frac{x^4y}{12} + \frac{x^5y}{60} - \frac{x^6}{120} + \frac{x^6y}{180}$$

$$Z = \phi_1(y) + \phi_2(y-x) + \frac{x^4y}{12} + \frac{x^5y}{60} - \frac{x^6}{120} + \frac{x^6y}{180}$$

$$(X) (D^2 + DD' - 6D'^2)z = x^2 \sin(x+y)$$

$$\text{A.E. } D \rightarrow m, D' \rightarrow 1$$

$$m^2 + m - 6 = 0$$

$$(m+3)(m-2) = 0$$

$$m = -3, m = 2$$

$$\text{C.F.} = \phi_1(y-3x) + \phi_2(y+2x)$$

Mar 10, 2023, 17:23

$$\text{P.I.} = \frac{1}{F(D, D')} e^{ix+iy} x^2$$

$$D \rightarrow D+i$$

$$P.I. = \frac{1}{D^2 - 1 + 2Di + DD' + D'i + D'i - 1 - 6D'^2 + 6 - 12D'i}$$

$$= \frac{1}{D^2 - 6D'^2 + 4 + DD' + D(2i+i) + D'(i-12i)}$$

$$= \frac{1}{D^2 - 6D'^2 + 4 + DD' + 3iD + 11iD'}$$

$$= \frac{1}{D^2} \left[1 - \left[\frac{4 - 11iD' - 6D'^2 + DD' + 3iD}{D^2} \right]^{-1} x^2 \right]$$

~~Imag. Part~~, $\frac{1}{D^2} \left[x^2 - \frac{1}{D^2} [4x^2 + 6ix] \right]$

$$= \frac{1}{D^2} \left[\frac{x^4}{12} - \frac{x^4}{3} - ix^3 \right]$$

Imaginary Part = $\boxed{-\frac{x^5}{20}i}$

$$Z = \phi_1(y-3x) + \phi_2(y+2x) - \frac{x^5}{20}$$